proofs/monad/state.v
@@ -1,0 +1,56 @@
+From Stdlib Require Import FunctionalExtensionality.
+From shift_reset.monad Require Import state.
+
+Lemma map_id {S A} (m : state S A) :
+  map (fun x => x) m = m.
+Proof.
+  cbv. destruct m as [m]. f_equal.
+  apply functional_extensionality. intros s.
+  destruct (m s) as [x s'].
+  reflexivity.
+Qed.
+
+Lemma map_comp {S A B C} (f : B -> C) (g : A -> B) (m : state S A) :
+  map f (map g m) = map (fun x => f (g x)) m.
+Proof.
+  cbv. f_equal.
+  apply functional_extensionality. intros s.
+  destruct m as [m].
+  destruct (m s) as [x s'].
+  reflexivity.
+Qed.
+
+Lemma pure_bind {S A B} (x : A) (f : A -> state S B) :
+  bind (pure x) f = f x.
+Proof. cbv. destruct (f x) as [m]. reflexivity. Qed.
+
+Lemma bind_pure {S A} (m : state S A) :
+  bind m pure = m.
+Proof.
+  cbv. destruct m as [m]. f_equal.
+  apply functional_extensionality. intros s.
+  destruct (m s) as [x s'].
+  reflexivity.
+Qed.
+
+Lemma bind_assoc {S A B C} (m : state S A) (f : A -> state S B) (g : B -> state S C) :
+  bind (bind m f) g = bind m (fun x => bind (f x) g).
+Proof.
+  cbv. f_equal.
+  apply functional_extensionality. intros s.
+  destruct m as [m].
+  destruct (m s) as [x s'].
+  reflexivity.
+Qed.
+
+Lemma get_put {S} :
+  @bind S S unit get put = @pure S unit tt.
+Proof. cbv. reflexivity. Qed.
+
+Lemma put_get {S} (s : S) :
+  appr (put s) get = appr (put s) (pure s).
+Proof. cbv. reflexivity. Qed.
+
+Lemma put_put {S} (s1 s2 : S) :
+  appr (put s1) (put s2) = put s2.
+Proof. cbv. reflexivity. Qed.
